stated proper edge coloring result and filled out more proofs

Vizing/Main.lean
@@ -6,21 +6,21 @@ section
 open Aux Graph EdgeColoring Fan Path
 
 variable
-  {n : Nat} (G : Graph n)
+  {n : Nat} {G : Graph n}
 
-def edgeColor (G : Graph n) : EdgeColoring (maxDegree G + 1) G :=
-  extend (toEdgeSet G) empty
-where extend (E : EdgeSet G) (C : EdgeColoring (maxDegree G + 1) G) :
+def extendColoring (E : EdgeSet G) (C : EdgeColoring (maxDegree G + 1) G)
+  (h : ∀ e ∈ E.val, color C e = none) :
   EdgeColoring (maxDegree G + 1) G :=
 match hE : E.val with
 | [] => C
-| (x, y) :: _ =>
+| (x, y) :: es =>
   have hterm : (remove E (x, y)).val.length < E.val.length := by
     unfold remove
     simp_rw [hE, List.cons_removeAll]
     simp [List.removeAll]
     grw [List.length_filter_le]
     omega
+  have h' : ∀ e ∈ (remove E (x, y)).val, color C e = none := by sorry
   let F := maximalFan C (by apply E.reprGraphAx; rw [hE]; exact List.mem_cons_self)
   let a := (freeColorsOn C (last F)).head (existsFreeColor C (by omega) (last F))
   let b := (freeColorsOn C x).head (existsFreeColor C (by omega) x)
@@ -32,15 +32,58 @@ match hE : E.val with
       constructor
       · simp [heq, b]
       · simp [a]
-    extend (remove E (x, y)) (rotateFan C F a aux)
+    let C' := (rotateFan C F a aux)
+    have h' : ∀ e ∈ (remove E (x, y)).val, color C' e = none := by
+      intro e he
+      have he' : e ∈ E.val := by
+        simp [remove, List.removeAll] at he
+        exact he.left
+      unfold C'
+      rw [← h e he']
+      apply Eq.symm; apply rotateFan_invariant
+      by_contra hc
+      simp [remove, List.removeAll] at h he
+      rcases hc with ⟨hc, hc'⟩ | ⟨hc, hc'⟩
+      · have := fan_colored_edges x y F e.2 hc' (by intro h; rw [← hc, ← h] at he; simp at he)
+        rw [← hc, h e.1 e.2 he'] at this
+        simp at this
+      · have := fan_colored_edges x y F e.1 hc' (by intro h; rw [← hc, ← h] at he; simp at he)
+        rw [← hc, color_symm, h e.1 e.2 he'] at this
+        simp at this
+    extendColoring (remove E (x, y)) (rotateFan C F a aux) h'
   else
     let P : Path C a b x := maximalPath C ha hb heq (by simp [b])
     let C' := invert (C := C) (x := x) ha hb heq (by simp [b])
     let F' := findSubfanWithColor C F C' P (by unfold P; apply invert_spec)
     have aux : edgeColorValid C' (x, last F') a := by
       sorry
-    extend (remove E (x, y)) (rotateFan C' F' a aux)
+    let C'' := (rotateFan C' F' a aux)
+    have h' : ∀ e ∈ (remove E (x, y)).val, color C'' e = none := by sorry
+    extendColoring (remove E (x, y)) C'' h'
 termination_by
   E.val.length
+
+theorem extendColoring_proper (E : EdgeSet G) (C : EdgeColoring (maxDegree G + 1) G)
+  (h : ∀ e ∈ E.val, color C e = none)
+  (e : Edge n) (h1 : e ∈ (toEdgeSet G).val)
+  (h2 : e ∉ E.val → (color C e).isSome) :
+  (color (extendColoring E C h) e).isSome := by
+  fun_induction extendColoring
+  · simp_all
+  · rename_i ih
+    apply ih
+    sorry
+  · rename_i ih
+    apply ih
+    sorry
+
+def mkEdgeColoring (G : Graph n) : EdgeColoring (maxDegree G + 1) G :=
+  extendColoring (toEdgeSet G) empty (by simp [color, empty])
+
+theorem mkEdgeColoring_proper :
+  ∀ e ∈ (toEdgeSet G).val, (color (mkEdgeColoring G) e).isSome := by
+  intro e h
+  unfold mkEdgeColoring
+  apply extendColoring_proper <;> simp_all
 
 end
