Vizing/InversionGuarantee.lean
@@ -10,6 +10,28 @@ variable
   {n c : Nat} {G : Graph n} (C : EdgeColoring c G)
   {x y : Vertex n} {a b : Color c}
 
+-- Maximality : all free colors on last vertex of fan are free on x
+
+theorem inversion_guarantee (F : Fan C x y)
+  {C' : EdgeColoring c G}
+  {P : Path C a b x}
+  (hC' : isInverted C C' P) :
+  ∃ i : Fin F.val.size, a ∈ freeColorsOn C' F.val[i] := by
+  by_cases h : ∃ j : Fin F.val.size, color C (x, F.val[j]) = a
+  rcases h with ⟨j, hj⟩
+  have : j.val > 0 := by
+    by_contra hc
+    simp at hc
+    simp [hc, F.firstElemAx] at hj
+    sorry
+  sorry
+  have aux1 : a ∈ freeColorsOn C x := by sorry
+  have aux2 : P.val = [x] := by sorry
+  have aux3 : C' = C := by sorry
+  rw [aux3]
+  use ⟨F.val.size - 1, (by simp; apply Array.size_pos_iff.mpr; exact F.nonemptyAx)⟩
+  sorry
+
 def findSubfanWithColor (F : Fan C x y)
   (C' : EdgeColoring c G)
   (P : Path C a b x)
@@ -44,11 +66,18 @@ def findSubfanWithColor (F : Fan C x y)
 theorem subfan_spec (F : Fan C x y)
   (C' : EdgeColoring c G)
   (P : Path C a b x)
-  (h : isInverted C C' P):
+  (h : isInverted C C' P)
+  (h2 : a ∈ freeColorsOn C (last F)) :
   a ∈ freeColorsOn C' (last (findSubfanWithColor C F C' P h)) := by
   simp [last]
+  by_cases hF : (findSubfanWithColor C F C' P h).val = F.val
+  simp_rw [hF]
+
+
+  sorry
+
   simp [findSubfanWithColor]
-  
+
 
 
   sorry
